\documentclass[12pt]{article}
\usepackage{amsmath}
\usepackage{amssymb}
\usepackage{tikz}

\begin{document}

\begin{tikzpicture}[scale=1]
\begin{scope}[every node/.style={circle,draw}, thick]
\coordinate (a) at (1,3);
\coordinate (b) at (-1,3);
\coordinate (c) at (-3,3);
\coordinate (d) at (-5,3);
\coordinate (e) at (-7,3);
\coordinate (f) at (-9,3);
\coordinate (g) at (-11,3);
\coordinate (h) at (-13,3);
\coordinate (i) at (-15,3);
\coordinate (j) at (-17,3);
\coordinate (k) at (-19,3);
\coordinate (l) at (-21,3);
\coordinate (m) at (-23,3);
\coordinate (n) at (-25,3);
\coordinate (o) at (-27,3);
\coordinate (p) at (-29,3);
\coordinate (q) at (-31,3);
\coordinate (r) at (-33,3);
\coordinate (s) at (-35,3);
\coordinate (t) at (-37,3);
\coordinate (u) at (-39,3);
\coordinate (v) at (-41,3);
\coordinate (w) at (-43,3);
\coordinate (x) at (-45,3);
\coordinate (y) at (-47,3);
\coordinate (z) at (-49,3);

\end{scope}
\begin{scope}[every edge/.style={draw}]
\draw (a) edge[bend left=40] node[left,align=center]{\scriptsize{$a$}}(b);
\draw (b) edge[bend left=40] node[left,align=center]{\scriptsize{$b$}}(c);
\draw (c) edge[bend left=40] node[left,align=center]{\scriptsize{$a$}}(d);
\draw (d) edge[bend left=40] node[left,align=center]{\scriptsize{$b$}}(e);
\draw (e) edge[bend left=40] node[left,align=center]{\scriptsize{$a$}}(f);
\draw (f) edge[bend left=40] node[left,align=center]{\scriptsize{$b$}}(g);
\draw (g) edge[bend left=40] node[left,align=center]{\scriptsize{$a$}}(h);
\draw (h) edge[bend left=40] node[left,align=center]{\scriptsize{$b$}}(i);
\draw (i) edge[bend left=40] node[left,align=center]{\scriptsize{$a$}}(j);
\draw (j) edge[bend left=40] node[left,align=center]{\scriptsize{$b$}}(k);
\draw (k) edge[bend left=40] node[left,align=center]{\scriptsize{$a$}}(l);
\draw (l) edge[bend left=40] node[left,align=center]{\scriptsize{$b$}}(m);
\draw (m) edge[bend left=40] node[left,align=center]{\scriptsize{$a$}}(n);
\draw (n) edge[bend left=40] node[left,align=center]{\scriptsize{$b$}}(o);
\draw (o) edge[bend left=40] node[left,align=center]{\scriptsize{$a$}}(p);
\draw (p) edge[bend left=40] node[left,align=center]{\scriptsize{$b$}}(q);
\draw (q) edge[bend left=40] node[left,align=center]{\scriptsize{$a$}}(r);
\draw (r) edge[bend left=40] node[left,align=center]{\scriptsize{$b$}}(s);
\draw (s) edge[bend left=40] node[left,align=center]{\scriptsize{$a$}}(t);
\draw (t) edge[bend left=40] node[left,align=center]{\scriptsize{$b$}}(u);
\draw (u) edge[bend left=40] node[left,align=center]{\scriptsize{$a$}}(v);
\draw (v) edge[bend left=40] node[left,align=center]{\scriptsize{$b$}}(w);
\draw (w) edge[bend left=40] node[left,align=center]{\scriptsize{$a$}}(x);
\draw (x) edge[bend left=40] node[left,align=center]{\scriptsize{$b$}}(y);
\draw (y) edge[bend left=40] node[left,align=center]{\scriptsize{$a$}}(z);

\draw (a) edge[bend left=40] node[above,align=center]{\scriptsize{$\lambda^{-3}$}}(b);
\draw (b) edge[bend left=40] node[above,align=center]{\scriptsize{$\lambda^{-2}$}}(c);
\draw (c) edge[bend left=40] node[above,align=center]{\scriptsize{$\lambda^{-3}$}}(d);
\draw (d) edge[bend left=40] node[above,align=center]{\scriptsize{$\lambda^{-4}$}}(e);
\draw (e) edge[bend left=40] node[above,align=center]{\scriptsize{$\lambda^{-3}$}}(f);
\draw (f) edge[bend left=40] node[above,align=center]{\scriptsize{$\lambda^{-4}$}}(g);
\draw (g) edge[bend left=40] node[above,align=center]{\scriptsize{$\lambda^{-3}$}}(h);
\draw (h) edge[bend left=40] node[above,align=center]{\scriptsize{$\lambda^{-4}$}}(i);
\draw (i) edge[bend left=40] node[above,align=center]{\scriptsize{$\lambda^{-3}$}}(j);
\draw (j) edge[bend left=40] node[above,align=center]{\scriptsize{$\lambda^{-4}$}}(k);
\draw (k) edge[bend left=40] node[above,align=center]{\scriptsize{$\lambda^{-3}$}}(l);
\draw (l) edge[bend left=40] node[above,align=center]{\scriptsize{$\lambda^{-4}$}}(m);
\draw (m) edge[bend left=40] node[above,align=center]{\scriptsize{$\lambda^{-3}$}}(n);
\draw (n) edge[bend left=40] node[above,align=center]{\scriptsize{$\lambda^{-4}$}}(o);
\draw (o) edge[bend left=40] node[above,align=center]{\scriptsize{$\lambda^{-3}$}}(p);
\draw (p) edge[bend left=40] node[above,align=center]{\scriptsize{$\lambda^{-4}$}}(q);
\draw (q) edge[bend left=40] node[above,align=center]{\scriptsize{$\lambda^{-3}$}}(r);
\draw (r) edge[bend left=40] node[above,align=center]{\scriptsize{$\lambda^{-4}$}}(s);
\draw (s) edge[bend left=40] node[above,align=center]{\scriptsize{$\lambda^{-3}$}}(t);
\draw (t) edge[bend left=40] node[above,align=center]{\scriptsize{$\lambda^{-4}$}}(u);
\draw (u) edge[bend left=40] node[above,align=center]{\scriptsize{$\lambda^{-3}$}}(v);
\draw (v) edge[bend left=40] node[above,align=center]{\scriptsize{$\lambda^{-4}$}}(w);
\draw (w) edge[bend left=40] node[above,align=center]{\scriptsize{$\lambda^{-3}$}}(x);
\draw (x) edge[bend left=40] node[above,align=center]{\scriptsize{$\lambda^{-4}$}}(y);
\draw (y) edge[bend left=40] node[above,align=center]{\scriptsize{$\lambda^{-3}$}}(z);

\draw (a) edge[bend right=40] node[right,align=center]{\scriptsize{$\lambda^{-3}$}}(b);
\draw (b) edge[bend right=40] node[right,align=center]{\scriptsize{$\lambda^{-4}$}}(c);
\draw (c) edge[bend right=40] node[right,align=center]{\scriptsize{$\lambda^{-3}$}}(d);
\draw (d) edge[bend right=40